LeanScratch/Semantics/L3/Stx.lean
@@ -2,13 +2,18 @@ import Mathlib.Data.Rel
 import Mathlib.Data.Finset.Basic
 import Mathlib.Tactic.Linarith.Frontend
 
-namespace L2
+namespace L3
 
+@[aesop safe [constructors, cases]]
 inductive Ty
   | bool
   | int
   | void
   | arrow (arg res : Ty)
+  | prod (a b : Ty)
+  | sum  (a b : Ty)
+
+  | ref (t : Ty)
 deriving DecidableEq, Repr
 
 inductive Op
@@ -16,6 +21,7 @@ inductive Op
   | gte
 deriving DecidableEq, Repr
 
+@[aesop safe [constructors, cases]]
 inductive Expr
   | bool (val : Bool)
   | int  (val : Int)
@@ -26,17 +32,29 @@ inductive Expr
   | eif    (cond t f : Expr)
   | ewhile (cond e   : Expr)
 
-  | assign (addr : String) (e : Expr)
-  | deref (addr : String)
+  | ref (t : Ty) (e : Expr)
+  | loc (t : Ty) (l : ℕ)
+
+  | assign (addr : Expr) (e : Expr)
+  | deref  (addr : Expr)
 
   | seq   (a b : Expr)
 
   | bvar (idx : ℕ)
   | abs (ty : Ty) (body : Expr)
-  | app (fn arg : Expr) -- ------> inference is decidable this is not needed
-                        -- FUN!: Implement unification and make this nicer
+  | app (fn arg : Expr)
+
   | letVal (t : Ty) (val body : Expr)
-  | letRecVal (t : Ty) (val body : Expr)
+
+  | pair (a b : Expr)
+  | fst (body : Expr)
+  | snd (body : Expr)
+
+  | inl (other : Ty) (body : Expr)
+  | inr (other : Ty) (body : Expr)
+  | case (scrutinee a b : Expr)
+  -- cant be fucked to deal with these rn
+  /- | letRecVal (t : Ty) (val body : Expr) -/
 deriving DecidableEq, Repr
 
 namespace Expr
@@ -47,24 +65,34 @@ inductive IsValue : Expr → Prop
   | skip : IsValue .skip
   | fn : IsValue (.abs ty body)
 
+  | pair : IsValue a → IsValue b → IsValue (.pair a b)
+  | inl : IsValue a → IsValue (.inl _ a)
+  | inr : IsValue a → IsValue (.inr _ a)
+  | loc : IsValue (.loc _ v)
+
 def bvarShift (shift skip : ℕ) : Expr → Expr
   | .bvar n => .bvar $ if n < skip then n else n + shift
   | .abs ty body => .abs ty (body.bvarShift shift skip.succ)
   | .letVal t val body =>
     .letVal    t (val.bvarShift shift skip     ) (body.bvarShift shift skip.succ)
-  | .letRecVal t val body =>
-    .letRecVal t (val.bvarShift shift skip.succ) (body.bvarShift shift skip.succ)
+
+  | .pair a b => .pair (a.bvarShift shift skip) (b.bvarShift shift skip)
+  | .fst body => .fst (body.bvarShift shift skip)
+  | .snd body => .fst (body.bvarShift shift skip)
+
+  | .case scrutinee a b => .case (scrutinee.bvarShift shift skip) (a.bvarShift shift skip.succ) (b.bvarShift shift skip.succ)
+  | .inl other body => .inl other (body.bvarShift shift skip)
+  | .inr other body => .inr other (body.bvarShift shift skip)
 
   | .app a b => .app (a.bvarShift shift skip) (b.bvarShift shift skip)
   | .seq a b => .seq (a.bvarShift shift skip) (b.bvarShift shift skip)
-  | .assign addr body => .assign addr (body.bvarShift shift skip)
+  | .assign addr body => .assign (addr.bvarShift shift skip) (body.bvarShift shift skip)
+  | .deref body       => .deref (body.bvarShift shift skip)
   | .ewhile c body => .ewhile (c.bvarShift shift skip) (body.bvarShift shift skip)
   | .eif c t f => .eif (c.bvarShift shift skip) (t.bvarShift shift skip) (f.bvarShift shift skip)
   | .op a o b => .op (a.bvarShift shift skip) o (b.bvarShift shift skip)
-  | x@(.deref _)
-  | x@(.skip)
-  | x@(.int _)
-  | x@(.bool _) => x
+
+  | x@(.ref _ _) | x@(.loc _ _) | x@(.skip) | x@(.int _) | x@(.bool _) => x
 
 def replace.bvar (bvarId idx_shift : ℕ) (replace : Expr) : Expr :=
   match compare bvarId idx_shift with
@@ -77,19 +105,24 @@ def replace (idx_shift : ℕ) (body repl : Expr) : Expr := match body with
   | .abs ty body => .abs ty (body.replace idx_shift.succ repl)
   | .letVal t val body =>
     .letVal    t (val.replace idx_shift      repl) (body.replace idx_shift.succ repl)
-  | .letRecVal t val body =>
-    .letRecVal t (val.replace idx_shift.succ repl) (body.replace idx_shift.succ repl)
+
+  | .pair a b => .pair (a.replace idx_shift repl) (b.replace idx_shift repl)
+  | .fst body => .fst (body.replace idx_shift repl)
+  | .snd body => .fst (body.replace idx_shift repl)
+
+  | .case scrutinee a b => .case (scrutinee.replace idx_shift repl) (a.replace idx_shift.succ repl) (b.replace idx_shift.succ repl)
+  | .inl other body => .inl other (body.replace idx_shift repl)
+  | .inr other body => .inr other (body.replace idx_shift repl)
 
   | .app a b => .app (a.replace idx_shift repl) (b.replace idx_shift repl)
   | .seq a b => .seq (a.replace idx_shift repl) (b.replace idx_shift repl)
-  | .assign addr body => .assign addr (body.replace idx_shift repl)
+  | .assign addr body => .assign (addr.replace idx_shift repl) (body.replace idx_shift repl)
+  | .deref body       => .deref (body.replace idx_shift repl)
   | .ewhile c body => .ewhile (c.replace idx_shift repl) (body.replace idx_shift repl)
   | .eif c t f => .eif (c.replace idx_shift repl) (t.replace idx_shift repl) (f.replace idx_shift repl)
   | .op a o b => .op (a.replace idx_shift repl) o (b.replace idx_shift repl)
-  | x@(.deref _)
-  | x@(.skip)
-  | x@(.int _)
-  | x@(.bool _) => x
+
+  | x@(.ref _ _) | x@(.loc _ _)  | x@(.skip) | x@(.int _) | x@(.bool _) => x
 
 def β : Expr → Expr → Expr := replace 0
 
