LeanScratch/CDS.lean
@@ -1,0 +1,151 @@
+import Mathlib.Data.Nat.PSub
+
+namespace ConcDisSys
+
+-- This is a very uncomputable definition, optimally we would be using Σ' over ∃
+-- since it would let us elim into Type but sadly we are unable to do this
+structure Network : Type 1 :=
+  -- The amout of nodes
+  -- The type of events
+  E : Type
+  N : Type
+
+  -- Nodes are a collection of functions that at every timestamp can possibly
+  -- emit some set of events
+  nodes : N → ℕ → Set E
+
+  -- Events are uniquely emitted by a single node. Following this another node
+  -- can re-emit said event to show it happened later but some finite amount
+  -- of time must have passed.
+  connective : ∀ e ts,
+    -- Either an event was emitted before
+    (∃ node, ∃ prev < ts, e ∈ nodes node prev) ∨
+    -- Or a node uniquely emitted an event
+    (∃ node, (e ∈ nodes node ts) ∧ ∀ node' ≠ node, e ∉ nodes node' ts) ∨
+    -- Or an event is not associated with the ts
+    (∀ node, e ∉ nodes node ts)
+
+  -- Every event must occur at least once
+  eventSaturation : ∀ e, ∃ ts node, e ∈ nodes node ts
+
+def FirstOccurence {nw : Network} (e : nw.E) (ts : ℕ) : Prop :=
+  (∃ node, e ∈ nw.nodes node ts) ∧
+  ∀ prev < ts, ∀ nodes, e ∉ nw.nodes nodes prev
+
+theorem FirstOccurence.unique
+    (f1 : FirstOccurence e t1)
+    (f2 : FirstOccurence e t2)
+    : t1 = t2 :=
+  match h : compare t1 t2 with
+  | .eq => Nat.compare_eq_eq.mp h
+  | .lt => by
+    rw [Nat.compare_eq_lt] at h
+    exact False.elim $ f2.2 _ h f1.1.choose f1.1.choose_spec
+  | .gt => by
+    rw [Nat.compare_eq_gt] at h
+    exact False.elim $ f1.2 _ h f2.1.choose f2.1.choose_spec
+
+theorem extractFirstOccurence
+    {nw : Network} {e : nw.E}
+    (end_nd : nw.N) (end_ts : ℕ)
+    (p : e ∈ nw.nodes end_nd end_ts)
+    (current_v : ℕ)
+    (hlt : current_v ≤ end_ts)
+    (ind_ih : ∀ t < current_v, ∀ nd, e ∉ nw.nodes nd t)
+    : Exists (FirstOccurence e) :=
+  match nw.connective e current_v with
+  | .inl ⟨nd, prev, plt, emitted⟩ => False.elim (ind_ih prev plt nd emitted)
+  | .inr (.inl ⟨nd, ⟨isEmitted, _⟩⟩) =>
+    ⟨current_v, ⟨⟨nd, isEmitted⟩, ind_ih⟩⟩
+  | .inr (.inr cont) =>
+    if h' : end_ts = current_v then by
+      subst h'
+      exact False.elim (cont _ p)
+    else
+      extractFirstOccurence end_nd end_ts p current_v.succ (by omega) (fun t h =>
+        if h : t = current_v then by
+          subst h
+          exact cont
+        else ind_ih t (by omega))
+termination_by end_ts - current_v
+decreasing_by
+· simp_wf
+  omega
+
+theorem hasFirstOccurence {nw : Network} (e : nw.E) : Exists (FirstOccurence e) := 
+  let ⟨ts, nd, p⟩ := nw.eventSaturation e
+  extractFirstOccurence nd ts p 0 (Nat.zero_le ts) (fun _ v => by contradiction)
+
+/-- info: 'ConcDisSys.hasFirstOccurence' depends on axioms: [propext, Quot.sound] -/
+#guard_msgs in #print axioms hasFirstOccurence
+
+def Network.happensBefore {nw : Network} (e1 e2 : nw.E) : Prop :=
+  ∃ z, ∃ n > 0, FirstOccurence e1 z ∧ FirstOccurence e2 (z + n)
+
+abbrev Network.concurrent {nw : Network} (e1 e2 : nw.E) : Prop :=
+  (¬happensBefore e1 e2) ∧ (¬happensBefore e2 e1)
+
+namespace Network
+
+variable (nw : Network)
+
+set_option quotPrecheck false in section
+scoped infixl:50 "≺" => nw.happensBefore
+scoped infixl:50 "∥" => nw.concurrent
+end
+
+-- ########################################################################
+-- ################################ Ex 8 ##################################
+-- ########################################################################
+
+theorem happensBefore.irrefl : ¬(a ≺ a) := by
+  by_contra h
+  rcases h with ⟨w1, diff, pgt, p1, p2⟩
+  have := FirstOccurence.unique p1 p2
+  omega
+
+theorem happensBefore.trans (h1 : a ≺ b) (h2 : b ≺ c) : a ≺ c := by
+  rcases h1 with ⟨w1, diff1, pgt1, p11, p12⟩
+  rcases h2 with ⟨w2, diff2, _,    p21, p22⟩
+  obtain rfl := FirstOccurence.unique p12 p21
+  exists w1
+  exists diff1 + diff2
+  rw [Nat.add_assoc] at p22
+  exact ⟨Nat.add_pos_left pgt1 diff2, p11, p22⟩
+
+-- ########################################################################
+-- ################################ Ex 9 ##################################
+-- ########################################################################
+
+theorem optionSpace (e1 e2 : nw.E) : e1 ≺ e2 ∨ e2 ≺ e1 ∨ e1 ∥ e2 := by
+  have ⟨w1, p1⟩ := hasFirstOccurence e1
+  have ⟨w2, p2⟩ := hasFirstOccurence e2
+  cases h : compare w1 w2
+  <;> simp only [Nat.compare_eq_eq, Nat.compare_eq_gt, Nat.compare_eq_lt] at h
+  · refine .inl ⟨w1, w2 - w1, by omega, p1, ?_⟩
+    rw [ ←Nat.add_sub_assoc (Nat.le_of_succ_le h) _,
+         Nat.add_comm,
+         Nat.add_sub_assoc (Nat.le_refl _) _,
+         Nat.sub_self,
+         Nat.add_zero]
+    exact p2
+
+  · subst h
+    refine .inr $ .inr ⟨?_, ?_⟩
+    <;> rintro ⟨ts, diff, hlt, p1', p2'⟩
+    · have eq1 := p1.unique p1'
+      have eq2 := p2.unique p2'
+      simp_all only [gt_iff_lt, add_right_eq_self, add_zero, Nat.lt_irrefl]
+    · have eq1 := p2.unique p1'
+      have eq2 := p1.unique p2'
+      simp_all only [gt_iff_lt, add_right_eq_self, add_zero, Nat.lt_irrefl]
+  · refine .inr $ .inl ⟨w2, w1 - w2, by omega, p2, ?_⟩
+    rw [ ←Nat.add_sub_assoc (Nat.le_of_succ_le h) _,
+         Nat.add_comm,
+         Nat.add_sub_assoc (Nat.le_refl _) _,
+         Nat.sub_self,
+         Nat.add_zero]
+    exact p1
+
+end ConcDisSys.Network
+
