LeanScratch/Semantics/L3/TySpec.lean
@@ -1,0 +1,88 @@
+import LeanScratch.Semantics.L3.Stx
+
+namespace L3
+
+-- We need to use our function call smeantics
+-- when we implement the typ signagure of L3 in this case
+@[aesop safe [constructors, cases]]
+inductive TySpec : List Ty → Expr → Ty → Prop
+  | bool : TySpec Γ (.bool _) .bool
+  | int  : TySpec Γ (.int  _) .int
+  | skip : TySpec Γ .skip     .void
+
+  | op_add : TySpec Γ e₁ .int →
+             TySpec Γ e₂ .int
+    → TySpec Γ (.op e₁ .add e₂) .int
+  | op_gte : TySpec Γ e₁ .int →
+             TySpec Γ e₂ .int
+    → TySpec Γ (.op e₁ .gte e₂) .bool
+
+  | eif : TySpec Γ scrutinee .bool →
+          TySpec Γ a t →
+          TySpec Γ b t
+    → TySpec Γ (.eif scrutinee a b) t
+  | ewhile : TySpec Γ' c .bool →
+             TySpec Γ' e .void
+    → TySpec Γ' (.ewhile c e) .void
+
+  | ref : TySpec Γ (.ref t _) t.ref
+  | loc : TySpec Γ (.loc t _) t.ref
+
+  | assign : TySpec Γ addr t.ref →
+             TySpec Γ e    t
+    → TySpec Γ (.assign addr e) .void
+  | deref : TySpec Γ addr t.ref
+    → TySpec Γ (.deref addr) t
+
+  | seq : TySpec Γ a .void → TySpec Γ b o
+      → TySpec Γ (.seq a b) o
+
+  | bvar : (Γ[idx]? = some w)
+      → TySpec Γ (.bvar idx) w
+  | abs : TySpec (argTy :: Γ) body retTy
+      → TySpec Γ (.abs argTy body) (.arrow argTy retTy)
+  | app : TySpec Γ fn (.arrow argTy retType) → TySpec Γ arg argTy
+      → TySpec Γ (.app fn arg) retType
+
+  | letVal : TySpec Γ expr argTy →
+             TySpec (argTy :: Γ) body retTy
+      → TySpec Γ (.letVal argTy expr body) (.arrow argTy retTy)
+
+  | pair : TySpec Γ a aTy →
+           TySpec Γ b bTy
+      → TySpec Γ (.pair a b) (.prod aTy bTy)
+  | fst : TySpec Γ a (.prod aTy bTy)
+      → TySpec Γ (.fst a) aTy
+  | snd : TySpec Γ a (.prod aTy bTy)
+      → TySpec Γ (.snd a) bTy
+
+  | inl : TySpec Γ a aTy
+      → TySpec Γ (.inl bty a) (.sum aTy bTy)
+  | inr : TySpec Γ b bTy
+      → TySpec Γ (.inl aty b) (.sum aTy bTy)
+  | case : TySpec Γ scrutinee (.sum aTy bTy) →
+           TySpec (aTy :: Γ) a t →
+           TySpec (bTy :: Γ) b t
+      → TySpec Γ (.case scrutinee a b) t
+
+theorem TySpec.unique (a : TySpec Γ e t) (b : TySpec Γ e t') : t = t' := by
+  /- aesop? -/
+  induction a generalizing t'
+  <;> cases b
+  <;> (try rfl)
+  case eif s a b ihs iha ihb s' a' b' => exact iha a'
+  case deref a ih a' => exact (Ty.ref.injEq _ _).mp $ ih a'
+  case seq a b iha ihb a' b' => exact ihb b'
+  case bvar a b => exact (Option.some.injEq _ _).mp $ a.symm.trans b
+  · sorry
+  · sorry
+  · sorry
+  · sorry
+  · sorry
+  · sorry
+  · sorry
+  · sorry
+  · sorry
+  · sorry
+  · sorry
+
