LeanScratch/Semantics/MuLang/Stx3.lean
@@ -1,0 +1,337 @@
+import Mathlib.Data.Nat.PSub
+import Mathlib.Data.Rel
+import Mathlib.Data.Vector.Basic
+import LeanScratch.ListUtils
+
+
+-- Inductive and broken datatypes,
+-- a type like μ 0 is not valid
+inductive MuTy : Type
+  | unit : MuTy
+  | bvar (idx : Nat)
+  | sum  (a b : MuTy)
+  | prod (a b : MuTy)
+  | μ (body : MuTy)
+
+mutual
+inductive MuTy.Valid : ℕ → MuTy → Prop
+  | unit : Valid n .unit
+  | bvar : idx < n → Valid n (.bvar idx)
+  | prod : Valid n a → Valid n b → Valid n (.prod a b)
+  | sum  : Valid n a → Valid n b → Valid n (.sum  a b)
+
+  | μ : Ind n.succ body → Valid n (.μ body)
+
+
+-- Not actually an inductivity requirement
+inductive MuTy.Ind : ℕ → MuTy → Prop
+  | unit : Ind n .unit
+  | bvar : idx ≤ 0 → idx < n → Ind n (.bvar idx)
+  | sum  : Valid n a → Valid n b → Ind n (.sum  a b)
+
+  | prod : Ind n a → Ind n b → Ind n (.prod a b)
+end
+
+mutual
+theorem MuTy.Ind.lower (hlt : n ≤ k) (prev : Ind n body) : Ind k body := match body, prev with
+  | .unit, _=> .unit
+  | .μ body, p => by cases p
+  | .prod a b, .prod ha hb => .prod (Ind.lower hlt ha) (Ind.lower hlt hb)
+  | .sum a b, .sum ha hb => .sum (Valid.lower hlt ha) (Valid.lower hlt hb)
+  | .bvar idx, .bvar ha hb => .bvar ha (Nat.lt_of_lt_of_le hb hlt)
+theorem MuTy.Valid.lower (hlt : n ≤ k) (prev : Valid n body) : Valid k body := match body, prev with
+  | .unit, _=> .unit
+  | .μ body, .μ hbody => .μ (Ind.lower (Nat.succ_le_succ hlt) hbody)
+  | .prod a b, .prod ha hb => .prod (Valid.lower hlt ha) (Valid.lower hlt hb)
+  | .sum a b, .sum ha hb => .sum (Valid.lower hlt ha) (Valid.lower hlt hb)
+  | .bvar idx, .bvar h => .bvar (Nat.lt_of_lt_of_le h hlt)
+end
+
+def MuTy.reduce (n : ℕ) : MuTy → MuTy → MuTy
+  | .unit, _ => .unit
+  | .μ body, r => .μ (body.reduce n.succ r)
+  | .prod a b, r => .prod (a.reduce n r) (b.reduce n r)
+  | .sum a b, r => .sum (a.reduce n r) (b.reduce n r)
+  | .bvar idx, r => match compare idx n with
+    | .lt => .bvar idx
+    | .eq => r
+    | .gt => .bvar idx.pred
+
+theorem MuTy.Valid_of_Ind (v : Ind n body) : Valid n body := match body, v with
+  | .bvar _ , .bvar _ a => .bvar a
+  | .prod _ _ , .prod ha hb => .prod (Valid_of_Ind ha) (Valid_of_Ind hb)
+  | .sum _ _, .sum ha hb => .sum ha hb
+  | .unit, _ => .unit
+
+-- Expresses types that have non-first class functions
+inductive Ty
+  | direct (body : MuTy) -- (h : body.Valid 0)
+  | arr    (arg  : MuTy) -- (h :  arg.Valid 0)
+           (ret : Ty)
+
+-- This type is valid but not inductive
+example : MuTy.Valid 0 (.μ (.sum (.bvar 0) (.bvar 0))) :=
+  .μ (.sum (.bvar Nat.one_pos) (.bvar Nat.one_pos))
+
+abbrev NatTy : MuTy := .μ (.sum .unit (.bvar 0))
+
+theorem NatTy.Valid : MuTy.Valid 0 NatTy := .μ (.sum .unit (.bvar Nat.one_pos))
+
+def MuTy.incrementExposed (skip inc : ℕ) : MuTy → MuTy
+  | .unit => .unit
+  | .μ body => .μ (body.incrementExposed skip.succ inc)
+  | .prod a b => .prod (a.incrementExposed skip inc) (b.incrementExposed skip inc)
+  | .sum a b => .sum (a.incrementExposed skip inc) (b.incrementExposed skip inc)
+  | .bvar idx => if idx < skip then .bvar idx else .bvar $ idx + inc
+
+theorem MuTy.increment_merge {t : MuTy}
+    : (t.incrementExposed skip a).incrementExposed skip b = t.incrementExposed skip (a + b)
+  := match t with
+  | .unit => rfl
+  | .bvar idx => by
+    dsimp [incrementExposed]
+    split
+    next h =>
+      simp only [
+        incrementExposed,
+        ite_eq_left_iff,
+        bvar.injEq,
+        add_right_eq_self]
+      intro x
+      exact False.elim (x h)
+    next h =>
+      dsimp [incrementExposed]
+      split
+      next h' =>
+        have : idx < skip := calc
+          idx ≤ idx + a := Nat.le_add_right idx a
+          _ < skip := h'
+        exact False.elim (h this)
+      · rw [Nat.add_assoc]
+  | .μ body => by
+    dsimp [incrementExposed]
+    rw [MuTy.increment_merge]
+  | .prod a b => by
+    dsimp [incrementExposed]
+    rw [increment_merge, increment_merge]
+  | .sum a b => by
+    dsimp [incrementExposed]
+    rw [increment_merge, increment_merge]
+
+@[simp]
+theorem MuTy.incrementExposed_zero : MuTy.incrementExposed skip 0 = id := by
+  funext x
+  induction x generalizing skip
+  <;> simp_all only [incrementExposed, add_zero, ite_self, id_eq]
+
+abbrev Ty.incrementExposed (skip inc : ℕ) : Ty → Ty
+  | .direct term => .direct (term.incrementExposed skip inc)
+  | .arr arg cont => .arr (arg.incrementExposed skip inc) (cont.incrementExposed skip inc)
+
+inductive Expr : Type
+  | unit
+  | lam (arg : MuTy) (body : Expr)
+  | app (fn arg : Expr)
+
+  | bvar (n : ℕ)
+  | fvar (n : ℕ)
+
+  | prod (a b : Expr)
+  | inl (other : MuTy) (body : Expr)
+  | inr (other : MuTy) (body : Expr)
+
+  -- At this point we need to increment each of the arguments bvars in some way
+  -- If this is not done the expression is false as the (.bvar 0) would refer to another type
+  | foldMu (t : MuTy) (body : Expr)
+  | unfoldMu (body : Expr)
+
+  | enterBMu (idx : ℕ) (body : Expr) 
+
+  | ematch (scrutinee a b : Expr)
+  | projl (body : Expr)
+  | projr (body : Expr)
+
+inductive TySpec (fΓ : List Ty) : /- bvar ctx -/ List MuTy → /- Γ ctx -/ List MuTy → Expr → Ty → Type
+  | unit : TySpec fΓ _ _ .unit (.direct .unit)
+  | lam : TySpec fΓ (argTy :: bvs) Γ body retTy
+      → TySpec fΓ bvs Γ (.lam argTy body) (.arr argTy retTy)
+  | app : TySpec _ bvs mΓ fn (.arr argTy retTy) → TySpec _ bvs mΓ arg (.direct argTy)
+      → TySpec _ bvs mΓ (.app fn arg) retTy
+
+  | bvar t : bvs[n]? = some t → TySpec fΓ bvs mΓ (.bvar n) (.direct t)
+  | fvar t :  fΓ[n]? = some t → TySpec fΓ bvs mΓ (.fvar n) t
+
+  | prod : TySpec _ bvs mΓ ea (.direct a) → TySpec _ bvs mΓ eb (.direct b)
+      → TySpec _ bvs mΓ (.prod ea eb) (.direct (.prod a b))
+  | inl : TySpec _ bvs mΓ body (.direct a)
+      → TySpec _ bvs mΓ (.inl b body) (.direct $ .sum a b)
+  | inr : TySpec _ bvs mΓ body (.direct b)
+      → TySpec _ bvs mΓ (.inr a body) (.direct $ .sum a b)
+
+  -- Rather than having increment exposed here, we can move it to only when we use the expr and then keep this static
+  | foldMu : TySpec _ bvs ((.μ body) :: mΓ) e (.direct body)
+      → TySpec _ bvs mΓ (.foldMu body e) (.direct (.μ body))
+  | unfoldMu : TySpec _ bvs mΓ e (.direct (.μ body))
+      → TySpec _ bvs mΓ (.unfoldMu e) (.direct (body.reduce 0 (.μ body)))
+
+  | enterBMu : mΓ[idx]? = some t → TySpec _ bvs mΓ body (.direct $ t.incrementExposed 0 idx)
+      → TySpec _ bvs mΓ (.enterBMu idx body) (.direct (.bvar idx))
+
+
+  | ematch : TySpec fΓ bvs mΓ scrutinee (.direct $ .sum a b) →
+             TySpec fΓ (a :: bvs) mΓ ea t →
+             TySpec fΓ (b :: bvs) mΓ eb t
+      → TySpec fΓ bvs mΓ (.ematch scrutinee ea eb) t
+
+  | projl : TySpec _ bvs mΓ body (.direct $ .prod a b)
+      → TySpec _ bvs mΓ (.projl body) (.direct a)
+  | projr : TySpec _ bvs mΓ body (.direct $ .prod a b)
+      → TySpec _ bvs mΓ (.projr body) (.direct b)
+
+theorem TySpec.unique (a : TySpec fΓ bvs mΓ expr t) (b : TySpec fΓ bvs mΓ expr t') : t = t' :=
+  match expr with
+  | .unit => match a, b with | .unit, .unit => rfl
+  | .lam ty body => match a, b with | .lam ax, .lam bx => (Ty.arr.injEq _ _ _ _).mpr ⟨rfl, TySpec.unique ax bx⟩
+  | .app fn arg => match a, b with | .app xa ya, .app xb yb => ((Ty.arr.injEq _ _ _ _).mp (TySpec.unique xa xb)).2
+
+  | .bvar n => match a, b with | .bvar _ a, .bvar _ b => (Ty.direct.injEq _ _).mpr $ (Option.some.injEq _ _).mp $ a.symm.trans b
+  | .fvar n => match a, b with | .fvar _ a, .fvar _ b => (Option.some.injEq _ _).mp $ a.symm.trans b
+
+  | .prod _ _ => match a, b with | .prod xa ya, .prod xb yb => (Ty.direct.injEq _ _).mpr
+    $ (MuTy.prod.injEq _ _ _ _).mpr ⟨(Ty.direct.injEq _ _).mp
+    $ TySpec.unique xa xb, (Ty.direct.injEq _ _).mp $ TySpec.unique ya yb⟩
+  | .inl _ _ => match a, b with | .inl a, .inl b => (Ty.direct.injEq _ _ ).mpr $ (MuTy.sum.injEq _ _ _ _).mpr ⟨(Ty.direct.injEq _ _).mp $ TySpec.unique a b, rfl⟩
+  | .inr _ _ => match a, b with | .inr a, .inr b => (Ty.direct.injEq _ _ ).mpr $ (MuTy.sum.injEq _ _ _ _).mpr ⟨rfl, (Ty.direct.injEq _ _).mp $ TySpec.unique a b⟩
+
+  | .foldMu t body => match a, b with | .foldMu a, .foldMu b => (Ty.direct.injEq _ _).mpr $ (MuTy.μ.injEq _ _).mpr rfl
+  | .unfoldMu body => match a, b with | .unfoldMu a, .unfoldMu b => (by rw [(MuTy.μ.injEq _ _).mp $ (Ty.direct.injEq _ _).mp $ TySpec.unique a b])
+
+  | .enterBMu idx body => match a, b with | .enterBMu _ a, .enterBMu _ b => rfl
+
+  | .ematch _ _ _ => match a, b with | .ematch as aa ab, .ematch bs ba bb => (by
+    obtain ⟨rfl, rfl⟩ := (MuTy.sum.injEq _ _ _ _).mp $ (Ty.direct.injEq _ _).mp $ TySpec.unique as bs
+    exact TySpec.unique aa ba)
+  | .projl body => match a, b with | .projl a, .projl b => (Ty.direct.injEq _ _).mpr ((MuTy.prod.injEq _ _ _ _).mp $ (Ty.direct.injEq _ _).mp $ TySpec.unique a b).1
+  | .projr body => match a, b with | .projr a, .projr b => (Ty.direct.injEq _ _).mpr ((MuTy.prod.injEq _ _ _ _).mp $ (Ty.direct.injEq _ _).mp $ TySpec.unique a b).2
+
+
+theorem TySpec.allEq (a b : TySpec fΓ bvs mΓ expr t) : a = b :=
+  match expr with
+  | .unit => match a, b with | .unit, .unit => rfl
+  | .lam ty body => match a, b with | .lam a, .lam b => (TySpec.lam.injEq _ _).mpr $ TySpec.allEq a b
+  | .app fn arg => match a, b with | .app xa ya , .app xb yb => (by
+    obtain ⟨rfl, _⟩ := (Ty.arr.injEq _ _ _ _).mp $ TySpec.unique xa xb
+    rw [TySpec.allEq xa xb, TySpec.allEq ya yb])
+
+  | .bvar n => match a, b with | .bvar _ _, .bvar _ _  => rfl
+  | .fvar n => match a, b with | .fvar _ _, .fvar _ _  => rfl
+
+  | .prod _ _ => match a, b with | .prod xa ya, .prod xb yb => (TySpec.prod.injEq _ _ _ _).mpr ⟨(TySpec.allEq xa xb), (TySpec.allEq ya yb)⟩
+  | .inl _ _ => match a, b with | .inl a, .inl b => (TySpec.inl.injEq _ _).mpr (TySpec.allEq a b)
+  | .inr _ _ => match a, b with | .inr a, .inr b => (TySpec.inr.injEq _ _).mpr (TySpec.allEq a b)
+
+  | .foldMu t body => match a, b with | .foldMu a, .foldMu b => (TySpec.foldMu.injEq _ _).mpr (TySpec.allEq a b)
+  | .unfoldMu body => sorry
+
+  | .enterBMu idx body => sorry
+
+  | .ematch scrutinee a b => sorry
+  | .projl body => sorry
+  | .projr body => sorry
+  /- | .unit => sorry -/
+  /- | .lam ty body => sorry -/
+  /- | .app fn arg => sorry -/
+
+  /- | .bvar n => sorry -/
+  /- | .fvar n => sorry -/
+
+  /- | .prod a b => sorry -/
+  /- | .inl a => sorry -/
+  /- | .inr a => sorry -/
+
+  /- | .foldMu body => sorry -/
+  /- | .unfoldMu body => sorry -/
+
+  /- | .enterBMu idx body => sorry -/
+
+  /- | .ematch scrutinee a b => sorry -/
+  /- | .projl body => sorry -/
+  /- | .projr body => sorry -/
+
+def Expr.bvarShift (skip shift : ℕ) : Expr → Expr
+  | .unit => .unit
+  | .lam ty body => .lam ty $ body.bvarShift skip.succ shift
+  | .app fn arg => .app (fn.bvarShift skip shift) (arg.bvarShift skip shift)
+
+  | .bvar n =>
+    if n < skip then .bvar n
+    else .bvar $ n + shift
+  | .fvar n => .fvar n
+
+  | .prod a b => .prod (a.bvarShift skip shift) (b.bvarShift skip shift)
+  | .inl b a => .inl b $ a.bvarShift skip shift
+  | .inr a b => .inr a $ b.bvarShift skip shift
+
+  | .foldMu t body => .foldMu t $ body.bvarShift skip shift
+  | .unfoldMu body => .unfoldMu $ body.bvarShift skip shift
+
+  | .enterBMu idx body => .enterBMu idx (body.bvarShift skip shift)
+
+  | .ematch scrutinee a b => .ematch (scrutinee.bvarShift skip shift) (a.bvarShift skip.succ shift) (b.bvarShift skip.succ shift)
+  | .projl body => .projl $ body.bvarShift skip shift
+  | .projr body => .projr $ body.bvarShift skip shift
+
+def TySpec.bvarShift
+    (prev : TySpec fΓ (bvs1 ++ bvs) mΓ e t)
+    : TySpec fΓ (bvs1 ++ bvs2 ++bvs) mΓ (e.bvarShift bvs1.length bvs2.length) t :=
+  match prev with
+  | .unit => .unit
+  | .lam body =>
+    let body : TySpec fΓ ((_ :: bvs1) ++ bvs) mΓ _ _ := body
+    .lam (body.bvarShift)
+  | .app fn arg =>
+    .app fn.bvarShift arg.bvarShift
+
+  | .bvar _ p => by
+    dsimp [Expr.bvarShift]
+    split
+    next h =>
+      apply TySpec.bvar
+      simp only [List.getElem?_append h, List.append_assoc] at p ⊢
+      exact p
+    next h => 
+      apply TySpec.bvar
+      simp only [not_lt] at h
+      simp only [List.append_assoc]
+      apply Eq.trans $ List.getElem?_append_right $ h.trans $ Nat.le_add_right _ _
+      rw [
+        Nat.sub_add_comm h,
+        List.getElem?_append_right (Nat.le_add_left _ _),
+        Nat.add_sub_cancel
+      ]
+      rw [List.getElem?_append_right h] at p
+      exact p
+  | .fvar _ p => .fvar _ p
+
+  | .prod a b => .prod a.bvarShift b.bvarShift
+  | .inl a => .inl a.bvarShift
+  | .inr a => .inr a.bvarShift
+
+  | .foldMu body => .foldMu body.bvarShift
+  | .unfoldMu body => .unfoldMu body.bvarShift
+
+  | .enterBMu idx body => .enterBMu idx body.bvarShift
+
+  | .ematch scrutinee a b =>
+    let a : TySpec fΓ ((_ :: bvs1) ++ bvs) mΓ _ _ := a
+    let b : TySpec fΓ ((_ :: bvs1) ++ bvs) mΓ _ _ := b
+    .ematch scrutinee.bvarShift a.bvarShift b.bvarShift
+  | .projl body => .projl body.bvarShift
+  | .projr body => .projr body.bvarShift
+
+-- benjamin peers types and programming langagues, equirecursive and isorecursive types
+-- Talk to : Mevan (french surname)
+
+/-- info: 'TySpec.bvarShift' depends on axioms: [propext] -/
+#guard_msgs in #print axioms TySpec.bvarShift
+
